local program eval

Code/Global to Session/DemoTest.lean
@@ -5,7 +5,7 @@ inductive DSL where
   | PLUS: DSL -> DSL -> DSL
 
 inductive MyOptional (t: Type): Type
-  | some (e: t): MyOptional t  
+  | some (e: t): MyOptional t
   | none: MyOptional t
 
 def eval: DSL -> MyOptional Nat
@@ -23,18 +23,86 @@ def eval: DSL -> MyOptional Nat
       | MyOptional.none => MyOptional.none
       | MyOptional.some v_b => MyOptional.some (v_a + v_b))
 
-
-
 def eval2: DSL -> Option Nat
   | DSL.CONSTANT n => (Option.some n)
   | DSL.DIVIDE a b => do
-    let v_a := <- eval2 a 
+    let v_a := <- eval2 a
     let v_b <- eval2 b
     if ( v_b == 0) then
       Option.none
     else (Option.some (v_a / v_b))
   | DSL.PLUS a b =>
     do
-    let v_a := <- eval2 a
-    let v_b := <- eval2 b
     Option.some ((<- eval2 a) + (<- eval2 b))
+
+
+--- Higher order Terms ---
+
+inductive Ty where
+| nat: Ty
+| string: Ty
+| fn: Ty -> Ty -> Ty
+
+@[reducible] def Ty.denote: Ty -> Type
+| nat => Nat
+| string => String
+| fn a b => a.denote -> b.denote
+
+inductive Term' (rep: Ty -> Type): Ty -> Type
+  | var           : rep x -> Term' rep x
+  | nat_const     : Nat -> Term' rep Ty.nat
+  | string_const  : String -> Term' rep Ty.string
+  | plus          : Term' rep Ty.nat -> Term' rep Ty.nat -> Term' rep Ty.nat
+  | my_let           : Term' rep x -> (rep x -> Term' rep y) -> Term' rep y
+  | lam           : (rep x -> Term' rep y) -> Term' rep (Ty.fn x y)
+  | app           : Term' rep (Ty.fn x y) -> Term' rep x -> Term' rep y
+
+def Term (ty: Ty) := {rep: Ty -> Type} -> Term' rep ty
+
+open Ty (nat fn)
+
+def add: Term (fn nat (fn nat nat)) :=
+  Term'.lam fun x => Term'.lam fun y => Term'.plus (Term'.var x) (Term'.var y)
+
+
+def three_test: Term nat :=
+  Term'.app (Term'.app add (Term'.nat_const 1)) (Term'.nat_const 4)
+
+#eval Nat.succ Nat.zero
+def countVars: Term' (fun _ => Unit) ty -> Nat
+  | .var _ => 1
+  | .nat_const _ => 0
+  | .string_const _ => 0
+  | .plus a b => countVars a + countVars b
+  | .app f a => countVars f + countVars a
+  | .lam b => countVars ( b ())
+  | .my_let a b => countVars a + countVars (b ())
+
+example : countVars add = 2 := rfl
+
+open Term'
+
+def pretty (e: Term' (fun _ => String) ty) (i: Nat := 1) : String :=
+  match e with
+  | .var s => s
+  | .nat_const n => toString n
+  | string_const s => s
+  | app f a => s!"({pretty f i} {pretty a i})"
+  | plus a b => s!"({pretty a i} + {pretty b i})"
+  | lam f     =>
+    let x := s!"x_{i}"
+    s!"(fun {x} => {pretty (f x) (i+1)})"
+  | my_let a b  =>
+    let x := s!"x_{i}"
+    s!"(let {x} := {pretty a i}; => {pretty (b x) (i+1)}"
+
+#eval pretty three_test
+
+#check three_test
+
+def length? {α : Type} (xs : List α) : Nat :=
+  match xs with
+  | [] => 0
+  | y :: ys => 1 + (length? ys)
+
+#eval length? [1,2,3,45,56]
