Code/Global to Session/Test/local_view.lean
@@ -1,54 +1,225 @@
 import Test.type
-import Test.agent
+import Test.location
 import Test.expression
+import Test.my_logs
+import Test.my_utils
 
-inductive LOCAL_PROGRAM where
-  | SEND    :  channelVarType -> variableType -> AGENT -> LOCAL_PROGRAM -> LOCAL_PROGRAM
-  | RECV    :  channelVarType -> variableType -> AGENT -> LOCAL_PROGRAM -> LOCAL_PROGRAM
-  | END     :   LOCAL_PROGRAM
-  | COMPUTE (v: variableType) (e: EXPRESSION) :   LOCAL_PROGRAM -> LOCAL_PROGRAM
- 
+namespace L
 
-inductive LOCAL_SESSION_TYPE where
-  | SEND    :  channelVarType -> variableType -> AGENT -> LOCAL_SESSION_TYPE -> LOCAL_SESSION_TYPE
-  | RECV    :  channelVarType -> variableType -> AGENT -> LOCAL_SESSION_TYPE -> LOCAL_SESSION_TYPE
-  | END     :  LOCAL_SESSION_TYPE
+  inductive P where
+    | IF      :  Variable -> EXPRESSION -> P -> P -> P -> P
+    | SEND    :  Variable -> Location -> P -> P
+    | RECV    :  Variable -> Location -> P -> P
+    | END     :  Option EXPRESSION -> P
+    | COMPUTE (v: Variable) (e: EXPRESSION) :   P -> P
+deriving BEq
 
-def LOCAL_TO_TYPE: LOCAL_PROGRAM -> LOCAL_SESSION_TYPE
-  | LOCAL_PROGRAM.SEND c v receiver p => LOCAL_SESSION_TYPE.SEND c v receiver (LOCAL_TO_TYPE p)
-  | LOCAL_PROGRAM.RECV c v sender p => LOCAL_SESSION_TYPE.RECV c v sender (LOCAL_TO_TYPE p)
-  | LOCAL_PROGRAM.COMPUTE _ _ p => (LOCAL_TO_TYPE p)
-  | LOCAL_PROGRAM.END => LOCAL_SESSION_TYPE.END
+  inductive T where
+    | IF      :  Variable -> T -> T -> T -> T
+    | SEND    :  Variable -> Location -> T -> T
+    | RECV    :  Variable -> Location -> T -> T
+    | END     :  T
 
-def LOCAL_PROGRAM_TO_STRING: LOCAL_PROGRAM -> String
-  | LOCAL_PROGRAM.SEND c v receiver p => 
-    "!(" ++ (AGENT_TO_STRING receiver) ++ ", " ++ v ++ ")" ++ "\n" ++ (LOCAL_PROGRAM_TO_STRING p)
-  | LOCAL_PROGRAM.RECV c v sender p => 
-    "?(" ++ (AGENT_TO_STRING sender) ++ ", " ++ v ++ ")" ++ "\n" ++ (LOCAL_PROGRAM_TO_STRING p)
-  | LOCAL_PROGRAM.COMPUTE v e p => v ++ " <= " ++ (EXPRESSION_TO_STRING e) ++ "\n" ++ (LOCAL_PROGRAM_TO_STRING p)
-  | LOCAL_PROGRAM.END => "END"
-
-def LOCAL_TYPE_TO_STRING: LOCAL_SESSION_TYPE -> String
-  | LOCAL_SESSION_TYPE.SEND c v receiver p => 
-    "!(" ++ (AGENT_TO_STRING receiver) ++ ", " ++ v ++ ")" ++ "\n" ++ (LOCAL_TYPE_TO_STRING p)
-  | LOCAL_SESSION_TYPE.RECV c v sender p => 
-    "?(" ++ (AGENT_TO_STRING sender) ++ ", " ++ v ++ ")" ++ "\n" ++ (LOCAL_TYPE_TO_STRING p)
-  | LOCAL_SESSION_TYPE.END => "END"  
-
-instance LOCAL_PROGRAM_DEBUG: ToString LOCAL_PROGRAM where 
-  toString := LOCAL_PROGRAM_TO_STRING
-
-instance: ToString LOCAL_SESSION_TYPE where 
-  toString := LOCAL_TYPE_TO_STRING
-
-def lp_1: LOCAL_PROGRAM := LOCAL_PROGRAM.SEND "channel1" "var1" AGENT.server LOCAL_PROGRAM.END
-def lp_2: LOCAL_PROGRAM := LOCAL_PROGRAM.SEND "channel1" "var1" AGENT.server
-  (LOCAL_PROGRAM.RECV "channel2" "var2" AGENT.server 
-  (LOCAL_PROGRAM.COMPUTE "var3" (EXPRESSION.CONSTANT 3) LOCAL_PROGRAM.END))
+  inductive eval_error where
+    | expression_error (e: EXPRESSION_RESULT Nat): eval_error
+    | unknown_message_var (name: Variable) : eval_error
+    | deadlock: eval_error
 
 
-#eval (lp_1)
-#eval (LOCAL_TO_TYPE lp_1)
+  abbrev msg := ((Location × Location)  × Variable) × Nat
 
-#eval (lp_2)
-#eval (LOCAL_TO_TYPE lp_2)
+  ---abbrev eval_res := ExceptT eval_error (StateT env (OptionT (with_logs String))) (Nat × (List msg))
+
+
+  inductive eval_res where
+  | finished  : Option Nat -> eval_res
+  | waiting   : eval_res
+
+  structure local_state where
+    env     : P_state
+    loc     : Location
+    prog    : P
+    ready   : Bool  := true
+
+  structure state where
+    messages: List msg
+    current : local_state
+    progs   : List (Location × local_state)
+
+  abbrev eval_resM := ExceptT eval_error (StateM state) eval_res
+
+end L
+
+open L
+section PROGRAM
+open P
+
+
+
+def LP_status_string (b: Bool) := if b then "ready" else "blocking"
+
+def LOCAL_TO_TYPE: P -> T
+  | IF v _ opt_1 opt_2 p => T.IF v (LOCAL_TO_TYPE opt_1) (LOCAL_TO_TYPE opt_2) (LOCAL_TO_TYPE p)
+  | SEND v receiver p => T.SEND v receiver (LOCAL_TO_TYPE p)
+  | RECV v sender p => T.RECV v sender (LOCAL_TO_TYPE p)
+  | COMPUTE _ _ p => (LOCAL_TO_TYPE p)
+  | END _ => T.END
+
+
+def LP_TO_STRING: P -> String
+  | IF v e opt_a opt_b p => v ++ " <= if " ++ toString e ++ "\n" ++ LP_TO_STRING opt_a ++ "\nelse\n" ++ LP_TO_STRING opt_b ++ "\nend if\n" ++ LP_TO_STRING p
+  | SEND v receiver p =>
+    v ++ "@" ++ receiver ++ " <= " ++ v ++  "@" ++ "local" ++ "\n" ++ (LP_TO_STRING p)
+  | RECV v sender p =>
+    v ++ "@" ++ "local" ++ " <= " ++ v ++  "@" ++ sender ++ "\n" ++ (LP_TO_STRING p)
+  | COMPUTE v e p => v ++ " <= " ++ (EXPRESSION_TO_STRING e) ++ "\n" ++ (LP_TO_STRING p)
+  | END res => "RETURN " ++ toString res
+
+
+def LT_TO_STRING: T -> String
+  | T.IF v opt1 opt2 p => "[]"
+  | T.SEND v receiver p =>
+    "!(" ++ receiver ++ ", " ++ v ++ ")" ++ "\n" ++ (LT_TO_STRING p)
+  | T.RECV v sender p =>
+    "?(" ++ sender ++ ", " ++ v ++ ")" ++ "\n" ++ (LT_TO_STRING p)
+  | T.END => "END"
+
+instance: ToString P where
+  toString := LP_TO_STRING
+
+instance: ToString T where
+  toString := LT_TO_STRING
+
+instance: ToString eval_res where
+  toString := fun x => match x with
+    | eval_res.finished r => toString r
+    | eval_res.waiting => "waiting..."
+
+instance: ToString eval_error where
+  toString := fun x => match x with
+    | eval_error.expression_error e => "expression error + " ++ toString e
+    | eval_error.unknown_message_var v => "unknown message var: " ++ v
+    | eval_error.deadlock => "Deadlock"
+
+instance: ToString local_state where
+  toString := fun x =>
+    x.loc ++ "(" ++ LP_status_string x.ready ++ "):\n" ++ toString x.env
+
+instance: ToString state where
+  toString := fun x =>
+    let state_strings := list_to_string_seperated_by (x.progs.map (fun x => toString x.snd))  "\n"
+   "messages:\n" ++ toString x.messages ++ "\nrunning:\n" ++ toString x.current ++ "\nothers:\n" ++ state_strings
+
+instance: ToString (Except eval_error eval_res × state) where
+  toString := fun x => match x.fst with
+    | Except.ok res =>  toString x.snd ++ "result: " ++ toString res
+    | Except.error e => toString x.snd ++ "error:" ++ toString e
+
+
+
+def swap_running_program (s: state): Option state :=
+  let canidates := s.progs.filter (fun x => x.snd.ready)
+  match canidates with
+  | [] => Option.none
+  | nc::_ =>
+    let without_new := s.progs.filter (fun x => x.fst != nc.fst)
+    let new_others := without_new.cons (s.current.loc, {s.current with ready := false})
+
+    Option.some {s with current := nc.snd, progs := new_others}
+
+
+def eval_local: eval_resM := do
+  let state <- get
+  let running_program := state.current.prog
+  let c_env := state.current.env
+
+  match running_program with
+  | IF v e opt_a opt_b p =>
+
+    let evaluation := eval_expression c_env e
+      match evaluation with
+      | EXPRESSION_RESULT.some r =>
+        let new_var_map: List (Variable × Nat) := (var_map c_env).concat (v, r)
+        let new_env: P_state := (new_var_map, (funcs c_env))
+        set { state with current := {state.current with env := new_env, prog := p} }
+        eval_local
+      | x => throw (eval_error.expression_error x)
+
+  | SEND v receiver p => do
+    let var_opt := (var_map c_env).lookup v
+    match var_opt with
+    | Option.some var =>
+      let new_message: msg := (((state.current.loc, receiver), v), var)
+      set { state with messages := state.messages.cons new_message, current := {state.current with prog := p}}
+      eval_local
+    | Option.none => throw (eval_error.unknown_message_var v)
+
+  | RECV v_name sender p => do
+    let v_opt := state.messages.lookup ((sender, state.current.loc), v_name)
+    match v_opt with
+    | Option.some v =>
+      let new_var_map: List (Variable × Nat) := (var_map c_env).concat (v_name, v)
+      let new_env: P_state := (new_var_map, (funcs c_env))
+      set { state with current := {state.current with env := new_env, prog := p} }
+      eval_local
+    | Option.none => return eval_res.waiting
+
+  | COMPUTE v e p => do
+    let evaluation := eval_expression c_env e
+    match evaluation with
+    | EXPRESSION_RESULT.some r =>
+      let new_var_map: List (Variable × Nat) := (var_map c_env).concat (v, r)
+      let new_env: P_state := (new_var_map, (funcs c_env))
+      set { state with current := {state.current with env := new_env, prog := p} }
+      eval_local
+    | x => throw (eval_error.expression_error x)
+
+  | END res_expr_opt =>
+    match res_expr_opt with
+    | Option.some res_expr => do
+      let state <- get
+      let evaluation := eval_expression state.current.env res_expr
+      match evaluation with
+      | EXPRESSION_RESULT.some r =>
+        return eval_res.finished r
+      | x => throw (eval_error.expression_error x)
+    | Option.none => do
+      let state <- get
+      let swap_state_opt := swap_running_program state
+      match swap_state_opt with
+      | Option.some swap_state =>
+        set swap_state
+        eval_local
+      | Option.none => throw eval_error.deadlock
+
+
+
+def lp_1_sending: P := P.SEND "var1" "server" (P.END Option.none)
+def lp_2_receiving: P := P.RECV "var1" "client"
+  (P.END (Option.some (EXPRESSION.VAR "var1")))
+
+def l_env_1: P_state := ([("var1", 101)], [])
+
+def lstate_1_send: local_state := { loc := "client", env := l_env_1, prog:= lp_1_sending }
+def lstate_1_receive: local_state := { loc := "server", env := empty_P_state, prog:= lp_2_receiving }
+
+
+def state_1_send_then_receive: state := {
+  messages:= [],
+  progs   := [("server", lstate_1_receive)],
+  current := lstate_1_send
+}
+
+def state_2_only_receive: state := {
+  messages:= [],
+  progs   := [("server", lstate_1_receive)],
+  current := lstate_1_send
+}
+
+#eval (lp_1_sending)
+#eval (LOCAL_TO_TYPE lp_1_sending)
+#eval (eval_local lp_1_sending state_1_send_then_receive)
+
+#eval (lp_2_receiving)
+#eval (LOCAL_TO_TYPE lp_2_receiving)
+#eval (eval_local lp_2_receiving state_2_receiving)
