Code/Global to Session/Test/my_utils.lean
@@ -1,0 +1,7 @@
+def list_to_string_seperated_by (l: List String) (s: String): String :=
+  match l with
+  | List.cons a as => a ++ s ++ (list_to_string_seperated_by as s)
+  | _ => ""
+
+def list_to_continuos_string (l: List String): String :=
+  list_to_string_seperated_by l ""
